[inversion] Lift inversion from SFL

inversion.lean
@@ -1,41 +1,298 @@
 module
 
-public meta import Lean.Elab.Tactic.ElabTerm
-public meta import Lean.Meta.Tactic.Generalize
+public meta import Lean.Elab.ConfigEval
+public meta import Lean.Elab.Tactic.RenameInaccessibles
+public meta import Lean.Elab.Tactic.Induction
 public meta import Lean.Meta.Tactic.Cases
-public meta import Lean.Meta.Tactic.Contradiction
+meta import all Lean.Meta.Tactic.Cases
+
+meta section
+
+namespace Lean.Parser
+open Tactic
+
+/-- Internal syntactic representation of a single inversion alternative. -/
+declare_syntax_cat invAlt
+syntax " | " caseArg " => " tacticSeq : invAlt
+
+/-- An inversion alternative matching one or more goal tags,
+  expanding to multiple single [invAlt]s. -/
+declare_syntax_cat invAlts
+syntax (" | " caseArg)+ " => " tacticSeq : invAlts
+
+/--
+  `inversion t` generalizes nonvariable indices of the type of `t` before invoking `cases t`,
+  then solves away contradictory generated goals.
+  `t` itself will also be generalized with a heterogeneous equality `heq`
+  if trying to generalize the indices produces an ill-typed result.
+  * If `inversion +clear t` is set, then `heq` will be `clear`ed from the context if present,
+    along with `t` if there are no dependencies on it.
+  * The form `inversion t with | tag₁ x ... => tac ... | ... | tagₙ z ... => tac ...` is supported,
+    similar to that of `cases` and `inversion`.
+-/
+syntax (name := inversion)
+  "inversion " optConfig ident (" with " (colGe invAlts)+)? : tactic
+
+end Lean.Parser
+
+namespace Lean.Meta
+
+/-- Given equations `eqs` in the local context of `mvarId`,
+  unify them using [Lean.Meta.unifyEq?],
+  but if unification fails, leave the equation in the context.
+  This means we should never get a "Dependent elimination failed" error.
+  While marked partial, this _should_ always terminate,
+  decreasing on the sum of the sizes of the terms of each equation.
+
+  Lifted from [Lean.Meta.Cases.unifyEqs]. -/
+partial def unifyEqs (eqs : List FVarId) (mvarId : MVarId) (subst : FVarSubst) (caseName? : Option Name) : MetaM (MVarId × FVarSubst) := withIncRecDepth do
+  match eqs with
+  | [] => return (mvarId, subst)
+  | eq :: eqs =>
+    let some { mvarId, subst, numNewEqs } ← Option.join <$> (observing? $ unifyEq? mvarId eq subst MVarId.acyclic caseName?)
+      | unifyEqs eqs mvarId subst caseName?
+    let (newEqs, mvarId) ← mvarId.introN numNewEqs
+    let eqs := eqs.map (Expr.fvarId! ∘ subst.get)
+    unifyEqs (newEqs.toList ++ eqs) mvarId subst caseName?
+
+/-- Lifted from [Lean.Meta.Cases.unifyCasesEqs]. -/
+def unifyCasesEqs (eqs : List FVarId) (subgoals : Array CasesSubgoal) : MetaM (Array CasesSubgoal) :=
+  subgoals.filterMapM fun s => do
+    let eqs := eqs.filterMap (Expr.fvarId? ∘ s.subst.get)
+    let (mvarId, subst) ← unifyEqs eqs s.mvarId s.subst s.ctorName
+    if (← mvarId.isAssignedOrDelayedAssigned) then return none
+    else return some { s with
+      mvarId := mvarId,
+      subst  := subst,
+      fields := s.fields.map (subst.apply ·)
+    }
+
+/-- Try to clear the given fvars from the local context of each subgoal,
+  using the subgoals' substitution mappings to find the fvars.
+
+  As with [MVarId.tryClearMany], the fvars must be in the order they appear in the context.  -/
+def casesClearMany (subgoals : Array CasesSubgoal) (fvarIds : Array FVarId) : MetaM (Array CasesSubgoal) :=
+  subgoals.mapM fun s => do
+    let fvarIds := fvarIds.filterMap (Expr.fvarId? ∘ s.subst.get)
+    let mvarId ← s.mvarId.tryClearMany fvarIds
+    return { s with mvarId }
+
+end Lean.Meta
 
 namespace Lean.Elab.Tactic
-open Meta
+open Meta Term
 
-elab "inversion " targetName:term : tactic => withMainContext do
-  let mvarId ← getMainGoal
-  let target ← elabTerm targetName none
-  let targetId := target.fvarId!
-  let targetName ← targetId.getUserName
-  let targetType ← inferType target
-  let targetType ← whnf targetType
-  let ⟨indName, args⟩ := targetType.getAppFnArgs
-  match ← isInductive? indName with
-  | some indVal =>
-    let indices := args.drop indVal.numParams
-    let nonvars := indices.filter (not ·.isFVar)
-    let genargs : Array GeneralizeArg :=
-      nonvars.map ({ expr := ·, hName? := some (← mkFreshUserName $ targetName.append `eq) })
-    let ⟨substs, _, mvarId⟩ ← mvarId.generalizeHyp genargs #[targetId]
-    let .some newTarget := substs.map.find? targetId
-      | throwTacticEx `inversion mvarId m!"failed to generalize argument"
-    mvarId.withContext do
-      let subgoals ← mvarId.cases newTarget.fvarId!
-      let subgoals := subgoals.map (·.mvarId)
-      let subgoals ← subgoals.filterM (not <$> ·.contradictionCore {})
-      replaceMainGoal $ subgoals.toList
-  | none =>
-    throwTacticEx `inversion mvarId
-      m!"target is not an inductive type{indentExpr targetType}"
+structure InversionConfig where
+  clear : Bool := false
 
-end Tactic
+declare_config_elab elabInversionConfig InversionConfig
 
-example (f : Nat → Nat) (n : Nat) (le : f n ≤ 0) : f n = 0 := by
-  -- cases le /- Dependent elimination failed: Failed to solve equation 0 = f n -/
-  inversion le; rfl
+open Cases in
+def inversionCore (h : FVarId) (config : InversionConfig) : TacticM (List CasesSubgoal) := withMainContext do
+  let goal ← getMainGoal
+  goal.withContext do
+    let some ctx ← mkCasesContext? h
+    | throwTacticEx `inversion goal "Target {Expr.fvar h} does not belong to an inductive type"
+    -- If the target's type isn't a predicate with indices, behave like `cases`
+    if ← hasIndepIndices ctx then
+      let subgoals ← inductionCasesOn goal h default ctx
+      let subgoals ← if config.clear
+        then casesClearMany subgoals #[h]
+        else pure subgoals
+      return subgoals.toList
+    -- Otherwise, use custom [unifyEqs] to not fail on unifying HEqs
+    else
+      let gis@⟨newGoal, _, newTarget, numEqs⟩ ← generalizeIndices goal h
+      let (newEqs, newGoal) ← newGoal.introN numEqs
+      let some targetEq := newEqs.back?
+      | throwTacticEx `inversion newGoal "Failed to generalize target"
+      let subgoals ← inductionCasesOn newGoal newTarget default ctx
+      let subgoals ← elimAuxIndices gis subgoals
+      let subgoals ← unifyCasesEqs newEqs.toList subgoals
+      let subgoals ← if config.clear
+        then casesClearMany subgoals #[h, targetEq]
+        else pure subgoals
+      return subgoals.toList
+
+open Parser Tactic in
+/-- Given an inversion alternative and a list of goals,
+  solve the tagged goal with the provided tactics,
+  throwing an error if the goal cannot be found or solved. -/
+def evalInvAlt (goals : List CasesSubgoal) (alt : TSyntax `invAlt) : TacticM (List MVarId) :=
+  match alt with
+  | `(invAlt| | $tag:ident $vars:binderIdent* => $tactics:tacticSeq) => do
+    if let some goal := goals.find? (matchTag tag.getId $ ·.ctorName.getD default) then
+      return [← trySolveGoal vars tactics goal.mvarId]
+    else throwError m!"Invalid alternative name `{tag.getId}`: {← errorMsg}"
+  | `(invAlt| | _ $vars:binderIdent* => $tactics:tacticSeq) => do
+    if !goals.isEmpty then
+      goals.mapM (trySolveGoal vars tactics ·.mvarId)
+    else throwErrorAt alt m!"Invalid wildcard alternative: {← errorMsg}"
+  | _ => throwErrorAt alt "Could not parse inversion alternative"
+where
+  matchTag (tag name : Name) : Bool :=
+    tag == name || tag.isPrefixOf name || tag.isSuffixOf name
+  trySolveGoal (vars : TSyntaxArray ``binderIdent) (tactics : TSyntax ``tacticSeq) (goal : MVarId) : TacticM MVarId := do
+    let goals ← renameInaccessibles goal vars >>= evalTacticAt tactics
+    unless goals.isEmpty do
+      reportUnsolvedGoals goals
+    return goal
+  errorMsg : TacticM MessageData := do
+    let goalMsgs := goals.filterMap (.ofName <$> ·.ctorName)
+    return if goals.isEmpty
+      then m!"There are no unhandled alternatives"
+      else m!"Expected {.orList goalMsgs}"
+
+@[tactic Lean.Parser.inversion, inherit_doc Lean.Parser.inversion]
+public meta def evalInversion : Tactic
+  | `(tactic| inversion $config $h:ident $[with $[$alts?:invAlts]*]?) => do
+    let config ← elabInversionConfig config
+    let mut goals ← inversionCore (← getFVarId h) config
+    if let some alts := alts? then
+      let expandedAlts ← Array.flatten <$> alts.mapM expandInvAlts
+      for alt in expandedAlts do
+        let solvedGoals ← evalInvAlt goals alt
+        goals := goals.filter (!solvedGoals.contains ·.mvarId)
+      unless goals.isEmpty do
+        reportUnsolvedGoals $ goals.map (·.mvarId)
+    replaceMainGoal $ goals.map (·.mvarId)
+  | stx => throwErrorAt stx "Could not parse inversion tactic"
+where expandInvAlts
+  | `(invAlts| $[| $args:caseArg]* => $tactics:tacticSeq) =>
+    args.mapM (`(invAlt| | $(·) => $tactics))
+  | stx => throwErrorAt stx "Could not parse inversion alternatives"
+
+end Lean.Elab.Tactic
+
+end -- meta section
+
+namespace Tests
+open Nat
+
+set_option autoImplicit false
+set_option pp.proofs true
+set_option pp.fieldNotation false
+
+/-- error: Dependent elimination failed: Failed to solve equation
+  0 = f n -/
+#guard_msgs(error) in
+example (f : Nat → Nat) (n : Nat) (leq : f n ≤ 0) : 0 = f n := by
+  cases leq
+
+example (f : Nat → Nat) (n : Nat) (leq : f n ≤ 0) : 0 = f n := by
+  -- cases leq /- Dependent elimination failed: Failed to solve equation 0 = f n -/
+  inversion leq; assumption
+
+example (f : Nat → Nat) (n : Nat) (leq : f n ≤ 0) : 0 = f n := by
+  inversion +clear leq; assumption
+
+/-- error: Unknown identifier `leq` -/
+#guard_msgs(error) in
+example (f : Nat → Nat) (n : Nat) (leq : f n ≤ 0) : 0 = f n := by
+  inversion +clear leq
+  guard_hyp leq
+
+example (f : Nat → Nat) (n : Nat) (leq : f n ≤ 0) : 0 = f n := by
+  inversion leq with
+  | refl heq eq =>
+    guard_hyp heq : leq ≍ le.refl
+    guard_hyp eq : 0 = f n
+    assumption
+
+/-- warning: declaration uses `sorry` -/
+#guard_msgs(warning) in
+example (f : Nat → Nat) (n m : Nat) (leq : f n ≤ f m) : f n = 0 := by
+  inversion leq with
+  | refl e _ | step k _ e _ =>
+    try rw [← eq]
+    sorry
+
+/-- error: Invalid wildcard alternative: There are no unhandled alternatives -/
+#guard_msgs(error) in
+example (f : Nat → Nat) (n m : Nat) (leq : f n ≤ f m) : f n = 0 := by
+  inversion +clear leq with
+  | refl e | step k _ e =>
+    try rw [← e]
+    sorry
+  | _ => sorry
+
+/-- error: Invalid alternative name `step`: There are no unhandled alternatives -/
+#guard_msgs(error) in
+example (f : Nat → Nat) (n m : Nat) (leq : f n ≤ f m) : f n = 0 := by
+  inversion +clear leq with
+  | _ e | step k _ e =>
+    try rw [← e]
+    sorry
+
+inductive The : ∀ {α}, α → Prop where
+  | mk : The zero
+
+/-- Case names should be the constructors' names -/
+example {x : Nat} (h : The x) : x = zero := by
+  inversion h with
+  | mk => rfl
+
+example (n m o : Nat) : [n, m] = [o, o] → [n] = [m] := by
+  intro h
+  inversion h; rfl
+
+inductive NoStutter {α : Type} : List α → Prop where
+  | nostutter0: NoStutter []
+  | nostutter1 n : NoStutter (n::[])
+  | nostutter2 a b r (hneq : a ≠ b) (h : NoStutter (b::r)) : NoStutter (a::b::r)
+
+/-- The last (only) case name need not be provided -/
+example : ¬ (NoStutter [3, 1, 1, 4]) := by
+  intro contra
+  inversion contra with | _ contra =>
+  inversion contra with | _ h _ =>
+  apply h
+  rfl
+
+inductive Vec α : Nat → Type where
+  | nil : Vec α 0
+  | cons {n} : α → Vec α n → Vec α (n + 1)
+
+/-- Inversion should work on indexed `Type`s as well -/
+example {α} (n : Nat) (v : Vec α (n + 1)) : ∃ hd tl, v = Vec.cons hd tl := by
+  inversion v with
+  | cons hd tl => exists hd, tl
+
+inductive Wec α : Nat → Type where
+  | nil : Wec α 0
+  | cons {n} (f : Nat → Nat) : α → Wec α n → Wec α (f n)
+
+/-- warning: declaration uses `sorry` -/
+#guard_msgs(warning) in
+example {α} (n : Nat) (v : Wec α (succ n)) :
+    ∃ hd tl, v = Wec.cons succ hd tl := by
+  inversion v with
+  | cons m f hd tl eq heq =>
+    guard_hyp eq : succ n = f m
+    guard_hyp heq : v ≍ Wec.cons f hd tl
+    sorry
+
+inductive EmptyRelation : Nat → Nat → Prop where
+
+/-- Inversion should still work on nonindexed `Prop`s -/
+example n m : ¬ EmptyRelation n m := by
+  intro contra; inversion contra
+
+/-- With `inductive.autoPromoteIndices` true (the default),
+  this is also a nonindexed `Prop`... -/
+inductive silly : Nat → Prop where
+| silly1 n (h : n > 1) : silly n
+| silly2 n (h : exists m, m * 2 = n) : silly n
+| silly3 n (h : exists m, n = m + 2) : silly n
+
+/-- ...and inversion should continue to work -/
+example {n} (h : silly n) : n ≠ 1 := by
+  inversion h <;> omega
+
+/-- Inversion should also work on nonindexed `Type`s -/
+example (n : Nat) : Nat := by
+  inversion n with
+  | zero => exact zero
+  | succ n' => exact n'
+
+end Tests
